# Algorithmics Homework 2
###### tags: `report` `algorithm`
```
ç¬¬ 7 çµ„
è³‡å·¥äºŒB 109502546 åŠ‰èªèŠ¯
è³‡å·¥äºŒB 109502549 å¾ç‘„ç³
è³‡å·¥äºŒB 109502550 è¨±ç­±æ•
è³‡å·¥äºŒB 109502551 è‘‰å®¹ç‘„
è³‡å·¥äºŒB 109502564 æ—å¥•è¾°
è³‡ç®¡äºŒA 109403020 ç‹å»·å‚‘
```

### Problem 1
Indicate, for each pair of expressions (A, B) in the table below, whether A is O, o, Î©, Ï‰, or Î˜ of B. Assume that k â‰¥ 1, Îµ > 0, and c > 1 are constants. Your answer should be in the form of the table with "yes" or "no" written in each box.

> $A = O(B)$
let T=Yes, F=No

||A|B|$O$|$o$|$\Omega$|$\omega$|$\Theta$|
|--|---|---|----|---|---|---|---|
|a|$\lg^k{n}$|$n^\epsilon$|T|T|F|F|F|
|b|$n^k$|$c^n$|T|T|F|F|F|
|c|$\sqrt{n}$|$n^{\sin{n}}$|F|F|F|F|F|
|d|$2^n$|$2^{n/2}$|F|F|T|T|F|
|e|$n^{\lg{c}}$|$c^{\ln{n}}$|F|F|T|T|F|
|f|$\lg{n!}$|$\lg(n^n)$|T|F|T|F|T|

note.
e. $c^{\ln{n}}=c^{\frac{\ln{n}\ln{c}}{\ln{c}}}=c^{\log_c{n}\ln{c}}=n^{\ln{c}} \rightarrow c>1 ,\lg{c}>\ln{c}$
f. $\lg{n!}=\lg{n(n-1)(n-2)...(1)}= \displaystyle\sum^n_{i=1}{\lg(x)}$
$\rightarrow\int^n_1{\lg(x)dx}\le\sum^n_{i=1}\limits{\lg(x)}\le \int^{n+1}_{1}\lg(x)dx$
$\rightarrow x\lg{x} \mid^n_1\le\displaystyle\sum^n_{i=1}{\lg(x)}\le x\lg{x} \mid^{n+1}_1$
$\rightarrow \lg{n!}=O(n\lg{n})$
<!--
ä¹¾ç‚ºå•¥å³é‚Šç©åˆ†ç‰¹åˆ¥è‚¥èª°æ•‘æˆ‘ä¸€ä¸‹
fixed [name=å¤§ä¿ ]
å“¦å“¦å¥½è®š
æ‰€ä»¥æ˜¯\displaystyleé‹å—
åº¦
cool
-->

### Problem 2 
Given two non-negative function $f, g$ (i.e. $f, g : N \to R^*$) such that $f\not= O(g)$, $f\not= \Theta (g)$, and $f\not= \Omega (g)$.

ç”±ç¬¬ä¸€é¡Œc.å¯å¾—ï¼š
$f(n)=\sqrt n$
$g(n)$è¦æ‰¾ä¸æœƒæ”¶æ–‚çš„ï¼Œå°±ä¸æœƒå½¢æˆupper bound, lower bound.
$g(n)=n^{\sin{n}}$
![](../img/HW2/1.png)


### Problem 3
a. Rank the following functions by order of growth; that is, find an arrangement $g_1, g_2, â€¦, g_{30}$ of the functions satisfying $g_1 = Î©(g_2), g_2 = Î©(g_3), â€¦, g_{29} = Î©(g_{30})$. Partition your list into equivalence classes such that functions $f(n)$ and $g(n)$ are in the same class if and only if $f(n) = \Theta (g(n))$.
![](../img/HW2/2.png)

b. Give an example of a single nonnegative function $f(n)$ such that for all functions $g_i(n)$ in part (a), $f(n)$ is neither $O(g_i(n))$ nor $\Omega(g_i(n))$.

#### a )
æˆ‘å€‘å¯ä»¥å°‡é€™äº›å‡½å¼ä¾å¢é•·å¿«æ…¢åˆ†æˆäº”å€‹é¡åˆ¥ï¼špower towerã€factorialã€exponentialã€polynomial & logarithmicã€constant & iterated logarithm.
(Let $\lg n = k \Rightarrow 2^k = n$.)

- power tower: $a^{a^{\dots^a}}$
	- $g_{1} = 2^{2^{n+1}} = 2^{2\cdot 2^{n}} = 4^{2^n}$
	- $g_{2} = 2^{2^n}$
- factorial: $n!$ã€$n^n$
	- $g_{3} = (n+1)! = (n+1)\cdot n!$
	- $g_{4} = n!$ 
- exponential: $k^n$
	- $g_{5} = e^n$
	- $g_{6} = n \cdot 2^n$
	- $g_{7} = 2^n$
	- $g_{8} = (\dfrac32)^n$
- polynomial & logarithmic: $n^k$ã€$\lg n$
	- $\Theta((\lg n)^{\lg n})$
		- $g_{9} = n^{\lg \lg n} \rightarrow^{(å–\lg)} \lg\lg n\cdot\lg n$
		- $g_{10} = (\lg n)^{\lg n} \rightarrow^{(å–\lg)} \lg n\cdot\lg\lg n$
		- $g_{11} = (\lg n)! \approx (\lg n)^{\lg n}$
	- $g_{12} = n^3$
	- $\Theta(n^2)$
		- $g_{13} = n^2$
		- $g_{14} = 4^{\lg n} = 4^k = 2^k\cdot 2^k = n^2$
	- $\Theta(n\lg n)$
		- $g_{15} = n\lg n$
		- $g_{16} = \lg (n!)$
	- $\Theta(n)$
		- $g_{17} = n$
		- $g_{18} = 2^{\lg n} = 2^k = n$
	- $g_{19} = (\sqrt2)^{\lg n} = (\sqrt2)^k = 2^{\frac k2} = n^\frac12 = \sqrt n$
	- $g_{20} = 2^{\sqrt{2\lg n}} \rightarrow^{(å–\lg)}\sqrt{2k}$
	- $g_{21} = \lg^2 n \rightarrow^{(å–\lg)}2\lg k$
	- $g_{22} = \ln n$
	- $g_{23} = \sqrt{\lg n}$
	- $g_{24} = \ln (\ln n)$ 
- constant & iterated logarithm: $c$ã€$\lg^* n$
	- $g_{25} = 2^{\lg^* n}\rightarrow^{(å–\lg)}\lg^* n$
	- $g_{26} = \lg^* n$
	- $g_{27} = \lg^* (\lg n) = \lg^* n - 1$
	- $g_{28} = \lg (\lg^* n)$
	- $\Theta(c)$
		- $g_{29} = n^{\frac1{\lg n}} = 2^{k \cdot \frac1k} = 2$
		- $g_{30} = 1$
#### b )
- åœ¨æ‰€æœ‰$g_i(n)$ä¸­å¢é•·é€Ÿç‡æœ€å¿«ç‚º$2^{2^{n+1}}$ï¼Œæœ€æ…¢ç‚º$1$
- $1+\sin n$ç‚ºä¸€åœ¨$0$ ~ $2$é–“éœ‡ç›ªä¹‹é€±æœŸå‡½æ•¸
- ä»¤$f(n) = (1+\sin n)\cdot 4^{4^{n}}$ï¼Œå‰‡ $f(n)$ æ»¿è¶³ $f(n) \notin O(g_i(n)) \cap f(n) \notin \Omega(g_i(n))$

<!-- å®³å¤§ä¿  a.m. 00:20
å®³å¤§ä¿  a.m. 12:20 -->
### Problem 4
Let $f(n)$ and $g(n)$ be asymptotically positive functions. Prove or disprove each of the following conjectures.
a. $f(n) = O(g(n))$ implies $g(n) = O(f(n))$.
b. $f(n) + g(n) = \Theta (min( f(n), g(n))$.
c. $f(n) = O(g(n))$ implies $\lg(f(n)) = O(\lg(g(n)))$, where $\lg(g(n)) \ge 1$ and $f(n) \ge 1$ for all sufficiently large n.
d. $f(n) = O(g(n))$ implies $2^{f(n)}= O(2^{g(n)})$.
e. $f(n) = O((f(n))^2)$.
f. $f(n) = O(g(n))$ implies $g(n)= \Omega (f(n))$.
g. $f(n) = \Theta (f(n/2))$.
h. $f(n) + o(f(n)) = \Theta (f(n))$.
i. $f(n) = \Theta (g(n))$ implies $f(n)/g(n)=c\not= 0$


#### a. $f(n) = O(g(n))$ implies $g(n) = O(f(n))$.

$f(n)=O(g(n)) \Rightarrow$ $f(n) \le cÂ·g(n)$
$\Rightarrow (n)\ge \dfrac{1}{c}g(n)\Rightarrow g(n)=\Omega (f(n))$

Ans: False

#### b.$f(n) + g(n) = \Theta (min( f(n), g(n)))$.

let $f(n)=n,\ g(n)=n^2$
$\Rightarrow f(n)\in \Theta(n), g(n)\in \Theta(n^2)$
$\Rightarrow f(n)+g(n) = n^2 + n \notin \Theta(min(f(n),g(n))) = \Theta(n)$

Ans:False

#### c. $f(n) = O(g(n))$ implies $\lg(f(n)) = O(\lg(g(n)))$, where $\lg(g(n)) \ge 1$ and $f(n) \ge 1$ for all sufficiently large n.

Let $f, g: N \to R^+$
$O(g(n))$ denote the set {$f(n): \exists \ n_0 \in N \ni \forall n \ge n_0, f(n) \le cï¼g(n)$}
$f(n) \le cï¼g(n)$
$lg(f(n)) \le \ lg(cï¼g(n)) \Rightarrow \lg c +\lg n)$ ï¼ˆå·²çŸ¥ï¼‰
If $c<1 \Rightarrow \lg c<0$

è©¦è­‰ $\lg(f(n)) \le \ dï¼\lg(g(n)) \leftrightarrow \lg(f(n)) \in O(\lg(g(n)))$
$d= \frac{\lg g(n)+\lg c}{\lg g(n)}=1+ \frac{\lg c}{\lg g(n)}$
$\because \lg g(n) \ge 1$
$\therefore 1+\frac{\lg c}{\lg g(n)} \le 1+\lg c$
$\Rightarrow \lg f(n) \le (1+\lg c)Â·\lg g(n)$
$\Rightarrow \lg f(n) \in O(\lg g(n))$

Ans: True

#### d. $f(n) = O(g(n))$ implies $2^{f(n)}= O(2^{g(n)})$.

Counter example: $f(n)=2n,\ g(n)=n$
$\Rightarrow 2^{2^n}=4^n \ne O(2^n)$

Ans: False

#### e. $f(n) = O((f(n))^2)$.
There is a counter example : $f(n)=\dfrac{1}{n}$.
$\to f^2(n) = \dfrac{1}{n^2}$
$\to \displaystyle\lim_{n\to\infty} \dfrac{f(n)}{f^2(n)}=n$ --- By definition, $f(n) \ne O((f(n))^2)$.

Ans: False

#### f. $f(n) = O(g(n))$ implies $g(n)= \Omega (f(n))$.
$f(n)=O(g(n))\to f(n) \le cÂ·g(n)\to g(n) \ge \dfrac{1}{c}Â·f(n)\to g(n)= \Omega (f(n))$.

Ans: True
#### g. $f(n) = \Theta (f(\dfrac{n}{2}))$.
There is a counter example: $f(n)=2^n\to f( \dfrac{n}{2})=2^\frac{n}{2}$
$\displaystyle\lim_{n\to\infty} \dfrac{f(n)}{f(\dfrac{n}{2})}= \displaystyle\lim_{n\to\infty} \dfrac{2^n}{2^\frac{n}{2}}=  \displaystyle\lim_{n\to\infty} 2^\frac{n}{2}=\infty$
By definition, $f(n) \ne \Theta (f(n/2))$

Ans: False
#### h. $f(n) + o(f(n)) = \Theta (f(n))$.
- let $g(n)=o(f(n))$, it means that $0\le g(n)\le cÂ·f(n)$
- $f(n) = \Theta (f(n))$ when $c_1Â·f(n)\le f(n)\le c_2Â·f(n)$
- $g(n)+f(n) = f(n)+o(f(n))=\Theta(f(n))$ because $c_1f(n)\le f(n)+g(n)\le (c+c_2)f(n)$

Ans: True

#### i. $f(n) = \Theta (g(n))$ implies $f(n)/g(n)=c\not= 0$

$f(n) = \Theta (g(n))$ means that $c_1Â·g(n)\le f(n)\le c_2Â·g(n),  \exists c_1, c_2\in R^+$

Counter example: $f(n)=\sin n+2,\ g(n)=1$
$\Rightarrow 1 \le f(n) \le 3$
$\Rightarrow 1Â·g(n) \le f(n) \le 3Â·g(n)$ which satisfies the definition of $f(n)=\Theta(g(n))$
However, $\displaystyle\lim_{n\to\infty} \dfrac{f(n)}{g(n)}=\sin n+2 \ne c$

Ans: False
### Problem 5
Solve the recurrence $T (n) = 2T (\sqrt {ğ‘›}) +1$ by making a change of variables. Your solution should be asymptotically tight. Do not worry about whether values are integral.

- $\text{let } n =2^m$
    $T(2^m)=2T(2^{\frac {m}{2}})+1$
    $let\ S(m)=T(2^m)$
    $S(m)=2S(m/2)+1$
    By master theorem($a=2,b=2,k=0$)
    $0<\log_22=1$
    $S(m)=T(2^m)=T(n)=\Theta (m)=\Theta(\lg n)$
    $T(n)=\Theta(\lg n)$
    

### Problem 6
Give asymptotic upper and lower bounds for $T(n)$ in each of the following recurrences. Assume that $T(n)$ is constant for $n\le 2$. Make your bounds as tight as possible, and justify your answers.
a. $T(ğ‘›) = 2ğ‘‡ (\dfrac{ğ‘›}{2}) + ğ‘›^3$
b. $ğ‘‡(ğ‘›) = ğ‘‡ (\dfrac{9ğ‘›}{10}) + ğ‘›$
c. $ğ‘‡(ğ‘›) = 16ğ‘‡ (\dfrac{ğ‘›}{4}) + ğ‘›^2$
d. $ğ‘‡(ğ‘›) = 7ğ‘‡ (\dfrac{ğ‘›}{3}) + ğ‘›^2$
e. $ğ‘‡(ğ‘›) = 7ğ‘‡ (\dfrac{ğ‘›}{2}) + ğ‘›^2$
f. $ğ‘‡(ğ‘›) = 2ğ‘‡ (\dfrac{ğ‘›}{4}) + \sqrt {n}$
g. $ğ‘‡(ğ‘›) = ğ‘‡(ğ‘› âˆ’ 1) + ğ‘›$
h. $ğ‘‡(ğ‘›) = ğ‘‡(\sqrt {ğ‘›}) + 1$

#### a. $ğ‘‡(ğ‘›) = 2ğ‘‡ (\dfrac{ğ‘›}{2}) + ğ‘›^3$
- By the master theorem
    $f(n)=n^3=\Theta (n^3)$ 
    $\because k=3\gt \log_{b}{a}=\lg{2}=1$
    $\Rightarrow a\cdot f(\dfrac{n}{b})=\dfrac{n^3}{4}<c\cdot n^3 =c\cdot f(n),\  \forall c>\dfrac14$
    $\therefore T(n)=\Theta (n^3)$  
#### b. $ğ‘‡(ğ‘›) = ğ‘‡ (\dfrac{9ğ‘›}{10}) + ğ‘›$
- By the master theorem
    $f(n)=n=\Theta (n)$ 
    $\because k=1\gt \log_{b}{a}=\log_{\frac{10}{9}}{1}$
    $\Rightarrow a\cdot f(\dfrac nb)=\dfrac{9n}{10}<c\cdot n=c\cdot f(n),\ \forall c>\dfrac 9{10}$
    $\therefore T(n)=\Theta (n)$

#### c. $ğ‘‡(ğ‘›) = 16ğ‘‡ (\dfrac{ğ‘›}{4}) + ğ‘›^2$
- By the master theorem
    $f(n)=n^2=\Theta (n^2)$ 
    $\because k=2\ =\ \log_{b}{a}=\log_{4}{16}=2$
    $\therefore T(n)=\Theta (n^2\lg n)$

#### d. $ğ‘‡(ğ‘›) = 7ğ‘‡ (\dfrac{ğ‘›}{3}) + ğ‘›^2$
- By the master theorem
    $f(n)=n^2=\Theta (n^2)$ 
    $\because k=2\gt \log_{b}{a}=\log_{3}{7}$
    $\Rightarrow a\cdot f(\dfrac nb)=7\cdot\dfrac {n^2}9<c\cdot n^2=c\cdot f(n),\ \forall c>\dfrac79$
    $\therefore T(n)=\Theta (n^2)$

#### e. $ğ‘‡(ğ‘›) = 7ğ‘‡ (\dfrac{ğ‘›}{2}) + ğ‘›^2$
- By the master theorem
    $f(n)=n^2=\Theta (n^2)$ 
    $\because k=2\lt \log_{b}{a}=\lg{7}$
    $\therefore T(n)=\Theta (n^{\lg{7}})$

#### f. $ğ‘‡(ğ‘›) = 2ğ‘‡ (\dfrac{ğ‘›}{4}) + \sqrt {n}$
- By the master theorem
    $f(n)=\sqrt {ğ‘›}=\Theta (\sqrt {ğ‘›})$ 
    $\because k = \dfrac{1}{2}\ =\ \log_{b}{a}=\log_{4}{2}=\dfrac{1}{2}$
    $\therefore T(n)=\Theta (\sqrt{n}\lg n)$

#### g. $ğ‘‡(ğ‘›) = ğ‘‡(ğ‘› âˆ’ 1) + ğ‘›$
$\begin{split}
ğ‘‡(ğ‘›) &= ğ‘‡(ğ‘› âˆ’ 1) + ğ‘› \\
    &=T(n-2)+(n-1)+n\\
    &=T(n-3)+(n-2)+(n-1)+n\\
    &...\\
    &=T(2)+3+4+5+...+(n-2)+(n-1)+n\\
    &=T(2)+\dfrac{(n+3)(n-2)}{2}\\
    &=\Theta (n^2)
\end{split}$
#### h. $ğ‘‡(ğ‘›) = ğ‘‡(\sqrt {ğ‘›}) + 1$
- Let $n=2^m,\ S(m)=T(2^m)$
    $S(m)=S(\dfrac{m}{2})+1$
    By the master theorem
    $f(n)=1=n^0$
    $\because k=0\ =\ \log_{b}{a}=\lg{1}=0$
    $\begin{split}
    \therefore S(m)&=\Theta (m^0\lg m)=\Theta (\lg m)\\
    T(n) &=S(\lg n)=\Theta (\lg \lg n)
    \end{split}$

### Problem 7
Give asymptotic upper and lower bounds for T(n) in each of the following recurrences.
Assume that T(n) is constant for sufficiently small n. Make your bounds as tight as possible, and justify your answers.
a. $ğ‘‡(ğ‘›) = 4ğ‘‡ (\dfrac{n}{3}) + n \lg n$
b. $ğ‘‡(ğ‘›) = 3ğ‘‡ (\dfrac{n}{3}) +\dfrac{n}{\lg n}$
c. $ğ‘‡(ğ‘›) = 4ğ‘‡ (\dfrac{n}{2}) + ğ‘›^2\sqrt{ğ‘›}$
d. $ğ‘‡(ğ‘›) = 3ğ‘‡ (\dfrac{n}{3}-2) +\dfrac{n}{2}$
e. $ğ‘‡(ğ‘›) = 2ğ‘‡ (\dfrac{n}{2}) +\dfrac{n}{\lg n}$
f. $ğ‘‡(ğ‘›) = ğ‘‡ (\dfrac{n}{2}) + ğ‘‡ (\dfrac{n}{4}) + ğ‘‡ (\dfrac{n}{8}) + ğ‘›$
g. $ğ‘‡(ğ‘›) = ğ‘‡(ğ‘› âˆ’ 1) +\dfrac{1}{n}$
h. $ğ‘‡(ğ‘›) = ğ‘‡(ğ‘› âˆ’ 1) + \lg n$
i. $ğ‘‡(ğ‘›) = ğ‘‡(ğ‘› âˆ’ 2) +\dfrac{1}{\lg n}$
j. $ğ‘‡(ğ‘›) = \sqrt{ğ‘›}ğ‘‡(\sqrt{ğ‘›}) + ğ‘›$
k. $ğ‘‡(ğ‘›) = \sqrt{ğ‘›}ğ‘‡(ğ‘› âˆ’ 1) + n$

a. $ğ‘‡(ğ‘›) = 4ğ‘‡ (\dfrac{n}{3}) + n \lg n$
- By master theorem
    $f(n)=n\lg n$
    $n^{\log_{3}4}\approx n^{1.26}$
    $f(n)=n\lg n=O(n^{1.26-\epsilon})\exists\epsilon>0$
    $\rightarrow T(n) = \Theta(n^{\log_{3}4})$
    
b. $ğ‘‡(ğ‘›) = 3ğ‘‡ (\dfrac{n}{3}) +\dfrac{n}{lgn}$
- Same as e and visualize the question with tree.
    $T(n)=9T(\dfrac{n}{9})+\ 3\times \dfrac{\frac{n}{3}}{\lg n/3}+\dfrac{n}{\lg n}$
    $T(n)=nT(1)+n\sum_{i=0}^{\log_3n}\limits \dfrac{1}{\log_3\frac{n}{3^i}}$
    $T(n)=\Theta(n(1+(\dfrac{1}{\log_33})+(\dfrac{1}{\log_39})+...+(\dfrac{1}{\log_3n}))$
    $T(n)=\Theta(n(1+1+(\dfrac{1}{2})+(\dfrac{1}{3})+...+(\dfrac{1}{\log_3n})))$
    Harmonic series
    $T(n)=\Theta(n(1+\sum_{i=1}^{\log_3n}\limits\dfrac{1}{i}))$
    $\rightarrow T(n)=\Theta(n\lg\lg n)$
    
c.  $ğ‘‡(ğ‘›) = 4ğ‘‡ (\dfrac{n}{2}) + ğ‘›^2\sqrt{ğ‘›}$
- By master theorem
    $f(n)=n^2\sqrt{n}$
    $n^{log_{2}4}=n^2$
    $f(n)=n^2\sqrt{n}=O(n^{2+\epsilon})\exists\epsilon>0$
    $\rightarrow T(n) = \Theta(n^{5/2})$
    
d.$ğ‘‡(ğ‘›) = 3ğ‘‡ (\dfrac{n}{3}-2) +\dfrac{n}{2}$
We can ignore the constant 2 in $T(\dfrac{n}{3}-2)$
- By master theorem
    $f(n)=\dfrac{n}{2}$
    $n^{\log_{3}3}=n$
    $f(n)=\dfrac{n}{2}=O(n)$
    $\rightarrow T(n)=\Theta(n\lg n)$
    
e.$ğ‘‡(ğ‘›) = 2ğ‘‡ (\dfrac{n}{2}) +\dfrac{n}{\lg n}$

  - By master theorem
       $f(n)=\dfrac{n}{\lg n}=\Theta(k)$ and $1=\log_ba$
      Assume and let $n^{1-\epsilon}$ Compare to $\dfrac{n}{\lg n}$and only  $\epsilon>0$
      $\dfrac{f(n)}{n^{1-\epsilon}}=\dfrac{n^\epsilon}{\lg n}$
       $\lim\limits_{n \to +\infty} \frac{n^\epsilon}{\lg n} \quad$ Through  Lâ€™HÃ´pitalâ€™s Rule    $\rightarrow \lim\limits_{n \to +\infty} \frac{\epsilon n^{\epsilon-1}}{\frac{1}{n}} \quad= +\infty$
      The function is  divergent ,so it means $k>\log_ba$. So,it is contradition with assumption.
      $\rightarrow$ Master theorem can't be used
      $T(n)=2ğ‘‡ (\dfrac{n}{2}) +\dfrac{n}{\lg n}$ 
      
      $T(n)=4T(\dfrac{n}{4})+2 \dfrac{\frac{n}{2}}{\lg \dfrac{n}{2}}+\dfrac{n}{\lg n}$
      $T(n)=nT(1)+\sum_{i=1}^{\lg n}\limits \dfrac{n}{\lg \frac {n}{2^i} }=nT(1)+n\sum_{i=1}^{\lg n}\limits\dfrac{1}{i }$
      $\rightarrow T(n)=\Theta(n\lg \lg n)$
      
      
f. $ğ‘‡(ğ‘›) = ğ‘‡ (\dfrac{n}{2}) + ğ‘‡ (\dfrac{n}{4}) + ğ‘‡ (\dfrac{n}{8}) + ğ‘›$
- guess $T(n) = \Theta(n)$
    - $T(n)= T(\dfrac{n}{2})+T(\dfrac{n}{4})+T(\dfrac{n}{8})+n$
    - $(\dfrac{cn}{2}+\dfrac{cn}{4}+\dfrac{cn}{8}+n)=\dfrac{7}{8}cn+n\leq cn\rightarrow O(n)(c\geq8)$
    - $(\dfrac{cn}{2}+\dfrac{cn}{4}+\dfrac{cn}{8}+n)=\dfrac{7}{8}cn+n\geq cn\rightarrow \Omega(n) (c\leq8)$
    C is constant , we can realize $\Omega(n)<T(n)<O(n)$
    - Prove the guess is right.
     $\rightarrow T(n)=\Theta(n)$

g.$ğ‘‡(ğ‘›) = ğ‘‡(ğ‘› âˆ’ 1) +\dfrac{1}{n}$
- $T(n)=T(n-1)+\dfrac{1}{n}$
    $T(n)=T(n-2)+\dfrac{1}{n-1}+\dfrac{1}{n}$
    $T(n)=\sum_{i=1}^{n}\limits \dfrac{1}{i}$
    ![](https://i.imgur.com/VCRys4E.png =200x)
    Through this picture.$\sum\limits_{i=1}^{n}\dfrac{1}{i}\geq \int_1^n\dfrac{1}{x}dx$
    $\int \dfrac{1}{x}dx=\ln x+C$
    $\rightarrow T(n)=\Theta(\lg n)$
    
h.$ğ‘‡(ğ‘›) = ğ‘‡(ğ‘› âˆ’ 1) + ğ‘™ğ‘”ğ‘›$
- Through Stirling's formula
 $ğ‘‡(ğ‘›) = ğ‘‡(ğ‘› âˆ’ 1) + ğ‘™ğ‘”ğ‘›$
    $T(n) = T(n-2)+\lg (n-1)+\lg n$
    $T(n)=\sum\limits_{i=1}^n\lg i=\lg n!\leq \lg n^n$
    $\rightarrow T(n)=\Theta(n\log n)$

i.$ğ‘‡(ğ‘›) = ğ‘‡(ğ‘› âˆ’ 2) +\dfrac{1}{\lg n}$
- $ğ‘‡(ğ‘›) = ğ‘‡(ğ‘› âˆ’ 2) +\dfrac{1}{\lg n}$
  $T(n)=T(n-4)+\dfrac{1}{\lg (n-2)}+\dfrac{1}{\lg n}$
  $T(n)=\sum\limits_{i=0}^{n/2-1}\dfrac{1}{\lg (n-2\times i)}=\sum\limits_{i=1}^{n/2}\dfrac{1}{\lg (2i)}$
  $\int{\dfrac{1}{\lg{x}}}dx=\ln 2 Li(x)=\Theta(\dfrac{n}{\lg n})$
  
j.$ğ‘‡(ğ‘›) = \sqrt{ğ‘›}ğ‘‡(\sqrt{ğ‘›}) + ğ‘›$
- $ğ‘‡(ğ‘›) = \sqrt{n}ğ‘‡(\sqrt{ğ‘›}) + ğ‘›$
    Let $n=2^k$
    $T(2^k)=2^{k/2}T(2^{k/2})+2^k$
    Dividing $2^k$ so $\dfrac{T(2^k)}{2^k}=\dfrac{T(2^{k/2})}{2^{k/2}}+1$
    Let $Q(k)=\dfrac{T(2^{k})}{2^k}$
    $Q(k)=Q(k/2)+1$
    So, $Q(k)$ can apply master theorem
    $Q(k)=Q(k/2)+1=\Theta(\lg k)$
    $\dfrac{T(2^k)}{2^k}=\dfrac{T(2^{k/2})}{2^{k/2}}+1=\Theta(\lg k)$
    $T(2^k)=T(2^{k/2})+2^k=\Theta(2^k \lg k)$
    $\rightarrow T(n)=\Theta(2^{\lg n}\lg \lg n)=\Theta(n\lg \lg n)$

k.$ğ‘‡(ğ‘›) = \sqrt{ğ‘›}ğ‘‡(ğ‘› âˆ’ 1) + n$
- $T(n) = \sqrt{n}T(n âˆ’ 1) + n$
     $T(n)=\sqrt{n(n-1)}T(n-2)+\sqrt n(n-1)+n$
     $T(n)=\sqrt{n(n-1)(n-2)}T(n-3)+\sqrt {n(n-1)}(n-2)+\sqrt n(n-1)+n$ 
     $T(n)=\sqrt{n(n-1)(n-2)(n-3)}T(n-4)+\sqrt {n(n-1)(n-2)}(n-3)\sqrt {n(n-1)}(n-2)+\sqrt n(n-1)+n$
      
     $T(n)=n+\sqrt n(n-1)+\sqrt{n(n-1)}(n-2)+.....+ \sqrt{n(n-1)(n-2)....(2)(1)}$
     $T(n)=\Theta(\sqrt{n!})$
    
    
    
    

- guess: $T(n) \ge  d_1 \sqrt{n!}$
        $\begin{split} T(n)&= \sqrt{n}T(n-1)+n\\
            &\ge  \sqrt{n}\cdot d_1\sqrt{(n-1)!}+n\\
            &= d_1\sqrt{n!}+n\\
            &\ge  d_1\sqrt{n!}\end{split}$
        
- guess: $T(n) \le  d_2 \sqrt{n!},$ 
        $T(n)-2T(n-1)=(\sqrt{n}T(n-1)+n)-2(\sqrt{n-1}T(n-2)+(n-1))$
        $\begin{split} T(n)&=(\sqrt{n}+2)T(n-1)+n-2\sqrt{n-1}T(n-2)-2(n-1)\\
        &\le(\sqrt{n}+2)d_2\sqrt{(n-1)!}+n-2\sqrt{n-1}d_2\sqrt{(n-2)!}-2(n-1)\\
        &= d_2\sqrt{n!}+n-2(n-1)\\
        &= d_2\sqrt{n!}-n+2\\
        &\le d_2\sqrt{n!},\ \forall n\ge 2\end{split}$
- $\because d_1\sqrt{n!}\le T(n)\le d_2\sqrt{n!}\ ,\ \exists d_1,\ d_2\in R^+\\
    \therefore \  T(n)=\Theta(\sqrt{n!})\ \text{is right}$
<!--é ­è…¦é¢¨æš´å¾Œçš„çµæœï¼Œé¡†é¡† 
ä¸çŸ¥é“å¯ä¸å¯ä»¥ç”¨QQ
     
     - In substitution method
          $T(n)=\sqrt{n}\sqrt{n-1}!+n$
          $\sqrt {n!}+n \leq d\sqrt {n!}$
          $1+\dfrac{n}{\sqrt{n!}}\leq d$


        guess: T(n)<= d \sqrt{n!}
        T(n)= sqrt{n}T(n-1)+n
            <= sqrt{n} d\sqrt{(n-1)!}+n
            
        
åŠ æ²¹ è…¦ç´°èƒå…¨æ²’äº†q å„å—¨ å°±æˆ‘å€‘åœ¨è©¦XDDDD åƒå®µå¤œï¼
-->
          

            
     
     
<!--     kennyåŠ æ²¹æˆ‘å€‘é‚„ä½ ç©ºé–“
     
whyqqè¦ä¸­é¢¨äº† ä½ ä¹Ÿæ˜¯å¾ˆéè¯¶ ä½ æ˜¯ä¸Šå¯¦é«”èª²çš„äººé¡å—4 è¦ä¸è¦ä¸‹æ¬¡æ›ä½ ç¶é¡Œç›®ã„š éƒ½å¯ä»¥å•Š å¥½è¯¶ 
Guest jennings who are you
<!--
å—¨Kenny 
å—¨Eric
æ—©å®‰
è«‹å•ä½ åˆ°åº•æ˜¯Ericé‚„æ˜¯Kenny
Eric qq
é‚£Kennyæ˜¯æ€éº¼ä¾†çš„XDDD
èªªä¾†è©±é•·Q_Q
å§”å±ˆå·´å·´
-->